generalize type classes to multiple params

Stlc/Classes.v
@@ -3,22 +3,19 @@ Require Import Metalib.LibLNgen.
 From Equations Require Import Equations.
 
 (***********************************************************************)
-(** * Notations *)
+(** * Operations *)
 (***********************************************************************)
 
 Class Syntax (e : nat -> Set) := {
-   (* 
-      To state the lemmas generically, we need to know 
-      the free variable constructor of the datatype.
-      (And use this overloaded term consistently through the 
-      definitions of the language.)
-    *)
     fv : forall {n}, e n -> vars ;
     size : forall {n}, e n -> nat ;
     weaken : forall {n}, e n -> e (S n) ;
     close : forall {n}, atom -> e n -> e (S n) ;
-    open  : forall {n}, e n -> e (S n) -> e n ;
-    subst : forall {n}, e n -> atom -> e n -> e n
+}.
+
+Class Subst (e : nat -> Set) (u : nat -> Set) `{Syntax e} `{Syntax u} := {
+    open  : forall {n}, u n -> e (S n) -> e n ;
+    subst : forall {n}, u n -> atom -> e n -> e n    
 }.
 
 (***********************************************************************)
@@ -29,7 +26,7 @@ Class Syntax (e : nat -> Set) := {
    perhaps automatically proven by a future version of LNgen. *)
    
 
-Class SyntaxTheory (exp : nat -> Set) (evar : forall {n}, atom -> exp n) `{H: Syntax exp } := {
+Class SyntaxTheory (exp : nat -> Set) `{H: Syntax exp} := {
 
    size_weaken : forall n (t : exp n), size (weaken t) = size t;
 
@@ -40,54 +37,89 @@ Class SyntaxTheory (exp : nat -> Set) (evar : forall {n}, atom -> exp n) `{H: Sy
    size_close : forall n (e1 : exp n) x1, 
       size (close x1 e1) = size e1;
 
-   size_open : (forall k (e1 : exp (S k)) (e2 : exp k),
-      size e1 <= size (open e2 e1));
-
-   size_open_var : (forall k (e : exp (S k)) x,
-      size (open (evar x) e) = size e);
-
    close_inj : (forall k (e1 : exp k) e2 x1,
       close x1 e1 = close x1 e2 ->
       e1 = e2);
 
-   close_open : (forall n1 (e1 : exp (S n1)) x1 ,
-      x1 `notin` fv e1 ->
-      close x1 (open (evar x1) e1) = e1);
+  close_weaken : (forall n1 (e1 : exp n1) x1,
+                      x1 `notin` fv e1 ->
+                      close x1 e1 = weaken e1);
 
-   open_close : (forall n1 (e1 : exp n1) x1,
-      open (evar x1) (close x1 e1) = e1);
+(*
+  fv_close := fv_exp_close_exp_wrt_exp;
+  fv_subst_fresh := fv_exp_subst_exp_wrt_exp_fresh;
+  fv_subst_lower := fv_exp_subst_exp_wrt_exp_lower;
+  fv_subst_notin := fv_exp_subst_exp_wrt_exp_notin;
+  fv_subst_upper := fv_exp_subst_exp_wrt_exp_upper; *)
 
-   open_inj : (forall n1 (e2 e1:exp (S n1)) x1,
-      x1 `notin` fv e2 ->
-      x1 `notin` fv e1 ->
-      open (evar x1) e2 = open (evar x1) e1 ->
-      e2 = e1);
 
    (* TODO: add more *)
-
-   subst_intro  : forall n (e1 : exp (S n)) (x1:atom) (e2 : exp n),
-      x1 `notin` fv e1 ->
-      open e2 e1 = subst e2 x1 (open (evar x1) e1) ;
-
-   subst_open_var : forall n1 (e2 : exp (S n1)) e1 x1 x2,
-        x1 <> x2 ->
-        open (evar x2) (subst (weaken e1) x1 e2) = 
-          subst e1 x1 (open (evar x2) e2)
    }.
 
 (* TODO: rewriting/hint database for the above lemmas. *)
 
 
+Class SubstTheory (exp : nat -> Set) (u : nat -> Set) (uvar : forall {n}, atom -> u n) `{H: Subst exp u} := {
+
+   size_open : (forall k (e1 : exp (S k)) (e2 :u k),
+      size e1 <= size (open e2 e1));
+
+   size_open_var : (forall k (e : exp (S k)) x,
+      size (open (uvar x) e) = size e);
+
+   close_open : (forall n1 (e1 : exp (S n1)) x1 ,
+      x1 `notin` fv e1 ->
+      close x1 (open (uvar x1) e1) = e1);
+
+   open_close : (forall n1 (e1 : exp n1) x1,
+      open (uvar x1) (close x1 e1) = e1);
+
+   open_inj : (forall n1 (e2 e1:exp (S n1)) x1,
+      x1 `notin` fv e2 ->
+      x1 `notin` fv e1 ->
+      open (uvar x1) e2 = open (uvar x1) e1 ->
+      e2 = e1);
+
+   open_weaken : (forall n1 (e2 : exp n1) e1,
+                     open e1 (weaken e2) = e2);
+
+   subst_intro  : forall n (e1 : exp (S n)) (x1:atom) (e2 : u n),
+      x1 `notin` fv e1 ->
+      open e2 e1 = subst e2 x1 (open (uvar x1) e1) ;
+
+   subst_open_var : forall n1 (e2 : exp (S n1)) e1 x1 x2,
+        x1 <> x2 ->
+        open (uvar x2) (subst (weaken e1) x1 e2) = 
+          subst e1 x1 (open (uvar x2) e2)
+  (* 
+  fv_open_lower := fv_exp_open_exp_wrt_exp_lower;
+  fv_open_upper := fv_exp_open_exp_wrt_exp_upper;
+  *)
+
+  }.
+
 Create HintDb syntax.
 
-Hint Rewrite (fun {e} {v} `{K:SyntaxTheory e v} => @close_open e v _ _) 
+(*
+Hint Rewrite (fun {e} {u} {v} `{K:SubstTheory e u v} => @close_open e u v _ _) 
   using solve [auto; try typeclasses eauto] : syntax.
 
-Hint Rewrite (fun {e} {v} `{K:SyntaxTheory e v} => @open_close e v _ _) 
+Hint Rewrite (fun {e} {u} {v} `{K:SubstTheory e u v} => @open_close e u v _ _) 
   using solve [auto; try typeclasses eauto] : syntax.
 
-Hint Rewrite (fun {e} {v} `{K:SyntaxTheory e v} => @subst_open_var e v _ _) 
+Hint Rewrite (fun {e} {u} {v} `{K:SubstTheory e u v} => @subst_open_var e u v _ _) 
   using solve [auto; try typeclasses eauto] : syntax.
+*)
+
+Hint Rewrite  @close_open
+  using solve [auto; try typeclasses eauto] : syntax.
+
+Hint Rewrite @open_close
+  using solve [auto; try typeclasses eauto] : syntax.
+
+Hint Rewrite @subst_open_var
+  using solve [auto; try typeclasses eauto] : syntax.
+
 
 (***********************************************************************)
 (** * Rewriting / tactics *)
