Stlc/Lec2.v
@@ -462,6 +462,9 @@ Qed.
         Use [simp subst] to simplify the substitution.
 *)
 
+Hint Rewrite  @subst_open_var 
+  using solve [auto; try typeclasses eauto] : syntax.
+
 Lemma typing_subst : forall (E F : ctx) e u S T (z : atom),
   typing (F ++ [(z,S)] ++ E) e T ->
   typing E u S ->
