Stlc/Lemmas.v
@@ -526,21 +526,42 @@ Ltac default_auto ::= auto; tauto.
 Ltac default_autorewrite ::= fail.
 
 #[global]
-Instance STE :  SyntaxTheory exp (@var_f) := {
+Instance STE :  SyntaxTheory exp := {
   size_weaken := size_exp_weaken_exp;
   fv_weaken := fv_exp_weaken_exp;
   size_min  := size_exp_min;
   size_close := size_exp_close_exp_wrt_exp;
+  close_inj := close_exp_wrt_exp_inj;
+  close_weaken := close_exp_wrt_exp_weaken_exp
+}.
+
+(*
+  fv_close := fv_exp_close_exp_wrt_exp; *)
+(* TODO: fill in the rest *)
+
+#[global]
+Opaque STE.
+
+#[global]
+Instance SSTE :  SubstTheory exp exp (@var_f) := {
   size_open := size_exp_open_exp_wrt_exp;
   size_open_var := size_exp_open_exp_wrt_exp_var;
-  close_inj := close_exp_wrt_exp_inj;
-  close_open := close_exp_wrt_exp_open_exp_wrt_exp;
   open_close := open_exp_wrt_exp_close_exp_wrt_exp;
   open_inj := open_exp_wrt_exp_inj;
+  close_open := close_exp_wrt_exp_open_exp_wrt_exp;
+  open_weaken := open_exp_wrt_exp_weaken_exp;
+(*
+  fv_open_lower := fv_exp_open_exp_wrt_exp_lower;
+  fv_open_upper := fv_exp_open_exp_wrt_exp_upper; 
+  fv_subst_fresh := fv_exp_subst_exp_wrt_exp_fresh;
+  fv_subst_lower := fv_exp_subst_exp_wrt_exp_lower;
+  fv_subst_notin := fv_exp_subst_exp_wrt_exp_notin;
+  fv_subst_upper := fv_exp_subst_exp_wrt_exp_upper; *)
+
   subst_intro := subst_exp_wrt_exp_intro;
   subst_open_var := subst_exp_open_exp_wrt_exp_var 
 }.
 (* TODO: fill in the rest *)
 
 #[global]
-Opaque Syntax_exp.
+Opaque SSTE.
